fol defs v.0.1

HybridFOL.thy
@@ -1,6 +1,15 @@
 theory HybridFOL imports Main
 begin
 
+primrec member where
+  \<open>member _ [] = False\<close> |
+  \<open>member m (n # A) = (m = n \<or> member m A)\<close>
+
+lemma member_iff [iff]: \<open>member m A \<longleftrightarrow> m \<in> set A\<close>
+  by (induct A) simp_all
+
+definition almostAgree where \<open>almostAgree G n w n' = (if n' = n then w else G n')\<close>
+
 datatype 'a hybr_form 
   =  Pro 'a 
   | Nom nat
@@ -9,40 +18,54 @@ datatype 'a hybr_form
   | Sat nat \<open>'a hybr_form \<close> 
   | Pos \<open>'a hybr_form \<close>
 
-fun hybr_semantics :: \<open>('c \<Rightarrow> 'c \<Rightarrow> bool) \<Rightarrow> ('c \<Rightarrow> 'a \<Rightarrow> bool) \<Rightarrow>
+primrec maxNom where
+  \<open>maxNom (Pro a) n = n\<close> |
+  \<open>maxNom (Nom n1) n2 = max n1 n2\<close> |
+  \<open>maxNom (HNeg p) n = maxNom p n\<close> |
+  \<open>maxNom (HCon p1 p2) n = maxNom p1 (maxNom p2 n)\<close> |
+  \<open>maxNom (Sat n1 p) n2 = maxNom p (max n1 n2)\<close> |
+  \<open>maxNom (Pos p) n = maxNom p n\<close>
+
+primrec hybr_semantics :: \<open>'c set \<Rightarrow> ('c \<Rightarrow> 'c \<Rightarrow> bool) \<Rightarrow> ('c \<Rightarrow> 'a \<Rightarrow> bool) \<Rightarrow>
                   (nat \<Rightarrow> 'c) \<Rightarrow> 'c \<Rightarrow> 'a hybr_form \<Rightarrow> bool\<close> where
-  \<open>hybr_semantics R V G w (Pro a) = V w a\<close> |
-  \<open>hybr_semantics R V G w (Nom n) = ((G n) = w)\<close> |
-  \<open>hybr_semantics R V G w (HNeg p) = (\<not> hybr_semantics R V G w p)\<close> |
-  \<open>hybr_semantics R V G w (HCon p1 p2) = (hybr_semantics R V G w p1 \<and> hybr_semantics R V G w p2)\<close> |
-  \<open>hybr_semantics R V G w (Sat n p) = hybr_semantics R V G (G n) p\<close> |
-  \<open>hybr_semantics R V G w (Pos p) = (\<exists>v. (R w v) \<and> (hybr_semantics R V G v p))\<close>
+  \<open>hybr_semantics W R V G w (Pro a) = V w a\<close> |
+  \<open>hybr_semantics W R V G w (Nom n) = ((G n) = w)\<close> |
+  \<open>hybr_semantics W R V G w (HNeg p) = (\<not> hybr_semantics W R V G w p)\<close> |
+  \<open>hybr_semantics W R V G w (HCon p1 p2) = (hybr_semantics W R V G w p1 
+                                         \<and>  hybr_semantics W R V G w p2)\<close> |
+  \<open>hybr_semantics W R V G w (Sat n p) = hybr_semantics W R V G (G n) p\<close> |
+  \<open>hybr_semantics W R V G w (Pos p) = (\<exists> v \<in> W. (R w v) \<and> (hybr_semantics W R V G v p))\<close>
 
 datatype 'a fol_form
   = Apply 'a nat
-  | R nat nat
+  | Rel nat nat
   | Eq nat nat 
   | FNeg \<open>'a fol_form\<close>
   | FCon \<open>'a fol_form\<close> \<open>'a fol_form\<close>
   | Ex nat \<open>'a fol_form\<close>
- 
-primrec member where
-  \<open>member _ [] = False\<close> |
-  \<open>member m (n # A) = (m = n \<or> member m A)\<close>
 
-lemma member_iff [iff]: \<open>member m A \<longleftrightarrow> m \<in> set A\<close>
-  by (induct A) simp_all
+primrec fol_semantics where
+  \<open>fol_semantics W R V G (Apply a n) = V (G n) a\<close> |
+  \<open>fol_semantics W R V G (Rel n1 n2) = R (G n1) (G n2)\<close> |
+  \<open>fol_semantics W R V G (Eq n1 n2) = ((G n1) = (G n2))\<close> |
+  \<open>fol_semantics W R V G (FNeg p) = (\<not> fol_semantics W R V G p)\<close> |
+  \<open>fol_semantics W R V G (FCon p1 p2) = (fol_semantics W R V G p1 \<and> fol_semantics W R V G p2)\<close> |
+  \<open>fol_semantics W R V G (Ex n p) = (\<exists> w \<in> W. fol_semantics W R V (almostAgree G n w) p)\<close>
 
-fun fol_semantics where
-  \<open>\<close>
-
-fun ST where
+primrec ST where
   \<open>ST n (Pro a) nxt = Apply a n\<close> |
   \<open>ST n1 (Nom n2) nxt = Eq n1 n2\<close> |
   \<open>ST n (HNeg p) nxt = FNeg (ST n p nxt)\<close> |
   \<open>ST n (HCon p1 p2) nxt = FCon (ST n p1 nxt) (ST n p2 nxt)\<close> |
   \<open>ST n1 (Sat n2 p) nxt = ST n2 p nxt\<close> |
-  \<open>ST n (Pos p) nxt = Ex nxt (FCon (R n nxt) (ST nxt p (Suc nxt)))\<close>
+  \<open>ST n (Pos p) nxt = Ex nxt (FCon (Rel n nxt) (ST nxt p (Suc nxt)))\<close>
+
+definition consistent where \<open>consistent W R G w \<equiv>
+  (\<forall> w1 w2. R w1 w2 \<longrightarrow> w1 \<in> W \<and> w2 \<in> W) \<and> (\<forall> w1. (\<exists> n. G n = w1) \<longrightarrow> w1 \<in> W) \<and> (w \<in> W)\<close>
+
+lemma main: \<open>hybr_semantics W R V G w p 
+ = fol_semantics W R V (almostAgree G (maxNom p 0 + 1) w) (ST (maxNom p 0 + 1) p (maxNom p 0 + 2))\<close>
+  sorry
 
 
 
